Update ilist examples

nola/examples/logic/verify/ilist_base.v
@@ -2,19 +2,20 @@
 
 From nola.examples.heap_lang Require Export notation.
 
-(** Calls [f] on the first [c] elements of the infinite list by [d] *)
-Definition siter : val :=
-  rec: "self" "f" "c" "l" :=
-    if: "c" = #0 then #() else "f" "l";; "self" "f" ("c" - #1) (! ("l" +ₗ #1)).
+(** Calls ["f"] on the first ["n"] elements of the infinite list *)
+Definition siter : val := rec: "self" "f" "n" "l" :=
+  if: !"n" = #0 then #() else
+    "f" "l";; "n" <- !"n" - #1;; "self" "f" "n" (! ("l" +ₗ #1)).
 
-(** Calls [iter] with a non-deterministic [c] *)
-Definition siter_nd : val := λ: "f" "l", siter "f" Ndnat "l".
+(** Calls [iter] with non-deterministically initialized ["n"] *)
+Definition siter_nd : val := λ: "f" "l",
+  let: "n" := ref Ndnat in siter "f" "n" "l".
 
 (** Forks [c] threads executing [siter_nd] *)
-Definition siter_nd_forks : val :=
-  rec: "self" "f" "c" "l" :=
-    if: "c" = #0 then #() else
-      Fork (siter_nd "f" "l");; "self" "f" ("c" - #1) "l".
+Definition siter_nd_forks : val := rec: "self" "f" "k" "l" :=
+  if: !"k" = #0 then #() else
+    Fork (siter_nd "f" "l");; "k" <- !"k" - #1;; "self" "f" "k" "l".
 
-(** Calls [siter_nd_forks] with a non-deterministic [c] *)
-Definition siter_nd_forks_nd : val := λ: "f" "l", siter_nd_forks "f" Ndnat "l".
+(** Calls [siter_nd_forks] with a non-deterministic ["k"] *)
+Definition siter_nd_forks_nd : val := λ: "f" "l",
+  let: "k" := ref Ndnat in siter_nd_forks "f" "k" "l".
